theories/Syntax/BinOps.v
@@ -273,11 +273,8 @@ Module bop.
     (* Having looked at the BinSec/Rel and Katamaran paper, I think it makes sense to require this to succeed for both sides *)
     (* TODO: Make sure that this is definitely a logical choice *)
     (* TODO: The pattern occurs here again *)
-    Definition eval_relop_valRel {σ} (op : RelOp σ) (rv1 rv2 : RelVal σ) : Coq.Init.Datatypes.option Datatypes.bool :=
-      match rv1 , rv2 with
-      | ty.SyncVal _ v1 , ty.SyncVal _ v2 => Some (eval_relop_val op v1 v2)
-      | _ , _ => None
-      end.
+    Definition eval_relop_valRel {σ} (op : RelOp σ) (rv1 rv2 : RelVal σ) : RelVal bool :=
+      liftBinOpRV (C := Val bool) (eval_relop_val op) (relValToRV rv1) (relValToRV rv2).
 
     Definition eval_relop_prop
       (* Force TypeDefKit into the context, so that the eval_relop_equiv lemma
@@ -294,14 +291,12 @@ Module bop.
       | bvult => fun v1 v2 => bv.ult v1 v2
       end.
 
+    Set Printing Implicit.
     Definition eval_relop_propRel
       (* Force TypeDefKit into the context, so that the eval_relop_equiv lemma
          below doesn't leave unsolved existentials when used in rewriting. *)
-      {TDF : TypeDefKit TDN} {σ} (op : RelOp σ) (rv1 rv2 : RelVal σ) : Coq.Init.Datatypes.option Prop :=
-      match rv1 , rv2 with
-      | ty.SyncVal _ v1 , ty.SyncVal _ v2 => Some (eval_relop_prop op v1 v2)
-      | _ , _ => None
-      end.
+      {TDF : TypeDefKit TDN} {σ} (op : RelOp σ) (rv1 rv2 : RelVal σ) : RV Prop :=
+      liftBinOpRV (eval_relop_prop op) (relValToRV rv1) (relValToRV rv2).
 
     Lemma eval_relop_val_spec {σ} (op : RelOp σ) (v1 v2 : Val σ) :
       reflect (eval_relop_prop op v1 v2) (eval_relop_val op v1 v2).
@@ -317,56 +312,12 @@ Module bop.
         - apply bv.ult_spec.
     Qed.
 
-    (* TODO: This conceptually not hard, but somehow I can't get it done. *)
-    (* One of the reasons is not knowing how to simplify reflect (a1 /\ a2) (b1 && b2) *) 
-    Definition eval_relop_val_specRel {σ} (op : RelOp σ) (v1 v2 : RelVal σ) :=
-      option.liftOption2 reflect (eval_relop_propRel op v1 v2) (eval_relop_valRel op v1 v2).
-
-    (* TODO: Bunch of stuff from Gemini that seems like a very plausible solution to state the spec when using options *)
-    (* Lemma 1: If eval_relop_val_specRel gives Some (reflect P true), then P is true. *)
-    Lemma eval_relop_val_specRel_gives_true_prop : forall {σ} (op : RelOp σ) (v1 v2 : RelVal σ),
-      forall (P_prime : Prop),
-        eval_relop_val_specRel op v1 v2 = Some (reflect P_prime true) ->
-        P_prime.
-    Proof.
-      intros σ op v1 v2 P_prime H_eq.
-      destruct v1; destruct v2; cbn in H_eq; try congruence.
-      inversion H_eq as [H0].
-      assert (reflect P_prime true).
-      { rewrite <- H0.
-        apply eval_relop_val_spec. }
-      inversion H.
-      assumption.
-    Qed.
-
-    (* Lemma 2: If eval_relop_val_specRel gives Some (reflect P false), then P is false. *)
-    Lemma eval_relop_val_specRel_gives_false_prop : forall {σ} (op : RelOp σ) (v1 v2 : RelVal σ),
-      forall (P_prime : Prop),
-        eval_relop_val_specRel op v1 v2 = Some (reflect P_prime false) ->
-        ~ P_prime.
-    Proof.
-      intros σ op v1 v2 P_prime H_eq.
-      destruct v1; destruct v2; cbn in H_eq; try congruence.
-      inversion H_eq as [H0].
-      assert (reflect P_prime false).
-      { rewrite <- H0. apply eval_relop_val_spec. }
-      inversion H.
-      assumption.
-    Qed.
-
-    (* Lemma 3: If eval_relop_val_specRel is None, it's because one of the inputs was None. *)
-    Lemma eval_relop_val_specRel_is_None : forall {σ} (op : RelOp σ) (v1 v2 : RelVal σ),
-        eval_relop_val_specRel op v1 v2 = None ->
-        eval_relop_propRel op v1 v2 = None \/ eval_relop_valRel op v1 v2 = None.
-    Proof.
-      intros σ op v1 v2 H_eq_None.
-      destruct v1; destruct v2; cbn in H_eq_None; try congruence; cbn; auto.
-    Qed.
-
     Lemma eval_relop_equiv {σ} (op : RelOp σ) (v1 v2 : Val σ) :
       eval_relop_prop op v1 v2 <-> eval_relop_val op v1 v2 = true.
     Proof. now destruct (eval_relop_val_spec op v1 v2). Qed.
 
+    (* TODO: Revisit this if we actually need it *)
+    (* Likely you can make a version for SyncVal and NonSyncVal separately *)
     (* Lemma eval_relop_equivRel {σ} (op : RelOp σ) (v1 v2 : RelVal σ) : *)
     (*   eval_relop_propRel op v1 v2 <-> eval_relop_valRel op v1 v2 = Some true. *)
     (* Proof. now destruct (eval_relop_val_specRel op v1 v2). Qed. *)
@@ -396,8 +347,31 @@ Module bop.
       | relop op                   => eval_relop_val op
       end.
 
+    (* TODO: Somehow phrase this a lifting to make the connection the eval for Val easier to see *) 
     Definition evalRel {σ1 σ2 σ3 : Ty} (op : BinOp σ1 σ2 σ3) : RelVal σ1 -> RelVal σ2 -> RelVal σ3 :=
-      ty.liftBinOp (eval op).
+      match op in BinOp σ1 σ2 σ3 return RelVal σ1 -> RelVal σ2 -> RelVal σ3 with
+      | plus                       => ty.liftBinOpRV Z.add
+      | times                      => ty.liftBinOpRV Z.mul
+      | minus                      => ty.liftBinOpRV Z.sub
+      | land                       => ty.liftBinOpRV Z.land
+      | and                        => ty.liftBinOpRV andb
+      | or                         => ty.liftBinOpRV orb
+      | pair                       => Datatypes.pair
+      | cons                       => List.cons
+      | shiftr                     => ty.liftBinOpRV bv.shiftr
+      | shiftl                     => ty.liftBinOpRV bv.shiftl
+      | append                     => app
+      | bvadd                      => ty.liftBinOpRV bv.add
+      | bvsub                      => ty.liftBinOpRV bv.sub
+      | bvmul                      => ty.liftBinOpRV bv.mul
+      | bvand                      => ty.liftBinOpRV bv.land
+      | bvor                       => ty.liftBinOpRV bv.lor
+      | bvxor                      => ty.liftBinOpRV bv.lxor
+      | bvapp                      => ty.liftBinOpRV bv.app
+      | bvcons                     => ty.liftBinOpRV (fun b bs => bv.cons b bs)
+      | update_vector_subrange s l => ty.liftBinOpRV (bv.update_vector_subrange s l)
+      | relop op                   => eval_relop_valRel op
+      end.
 
   End WithTypes.
   #[export] Existing Instance eq_dec_binop.
