theories/Syntax/TypeDecl.v
@@ -29,7 +29,13 @@
 From Coq Require Import
      Bool.Bool
      Strings.String
-     ZArith.BinInt.
+     ZArith.BinInt
+     List
+     Classes.Morphisms
+     Classes.Morphisms_Prop
+     Classes.RelationClasses
+     Program.Basics
+.
 From Equations Require Import
      Equations.
 From Katamaran Require Import
@@ -70,7 +76,7 @@ Module ty.
     | string
     | list (σ : Ty)
     | prod (σ τ : Ty)
-    | sum  (σ τ : Ty)
+    (* | sum  (σ τ : Ty) *)
     | unit
 (*    | enum (E : enumi) *)
     | bvec (n : nat)
@@ -83,7 +89,7 @@ Module ty.
 
 
     (* convenience definition. *)
-    Definition option : Ty -> Ty := fun T => sum T unit.
+    (* Definition option : Ty -> Ty := fun T => sum T unit. *)
 
     Section Ty_rect.
       Variable P : Ty -> Type.
@@ -93,7 +99,7 @@ Module ty.
       Hypothesis (P_string : P string).
       Hypothesis (P_list   : forall σ, P σ -> P (list σ)).
       Hypothesis (P_prod   : forall σ τ, P σ -> P τ -> P (prod σ τ)).
-      Hypothesis (P_sum    : forall σ τ, P σ -> P τ -> P (sum σ τ)).
+      (* Hypothesis (P_sum    : forall σ τ, P σ -> P τ -> P (sum σ τ)). *)
       Hypothesis (P_unit   : P unit).
 (*      Hypothesis (P_enum   : forall E, P (enum E)). *)
       Hypothesis (P_bvec   : forall n, P (bvec n)).
@@ -108,7 +114,7 @@ Module ty.
         | string   => ltac:(apply P_string)
         | list σ   => ltac:(apply P_list; auto)
         | prod σ τ => ltac:(apply P_prod; auto)
-        | sum σ τ  => ltac:(apply P_sum; auto)
+        (* | sum σ τ  => ltac:(apply P_sum; auto) *)
         | unit     => ltac:(apply P_unit; auto)
 (*        | enum E   => ltac:(apply P_enum; auto) *)
         | bvec n   => ltac:(apply P_bvec; auto)
@@ -142,146 +148,383 @@ Module ty.
       | string => String.string
       | list σ' => Datatypes.list (Val σ')
       | prod σ1 σ2 => Val σ1 * Val σ2
-      | sum σ1 σ2 => Val σ1 + Val σ2
+      (* | sum σ1 σ2 => Val σ1 + Val σ2 *)
       | unit => Datatypes.unit
-(*      | enum E => enumt E *)
       | bvec n => bv n
-(*      | tuple σs => EnvRec Val σs
-      | union U => uniont U
-      | record R => recordt R *)
       end%type.
 
-      Inductive RelVal {TDC : TypeDeclKit} {TDN : TypeDenoteKit TDC} (τ : Ty) : Set :=
-      | SyncVal : Val τ -> RelVal τ
-      | NonSyncVal : Val τ -> Val τ -> RelVal τ
-      .
+    (* Inductive RelVal {TDC : TypeDeclKit} {TDN : TypeDenoteKit TDC} (τ : Ty) : Set := *)
+    (* | SyncVal : Val τ -> RelVal τ *)
+    (* | NonSyncVal : Val τ -> Val τ -> RelVal τ *)
+    (* . *)
 
-      Context {TDC : TypeDeclKit}.
-      Context {TDN : TypeDenoteKit TDC}.
+    Set Universe Polymorphism.
+    Inductive RV (A : Type) : Type :=
+    | SyncVal : A -> RV A
+    | NonSyncVal : A -> A -> RV A
+    .
 
-      Definition projLeft {σ} (rv : RelVal σ) : Val σ :=
-        match rv with
-        | SyncVal _ v => v
-        | NonSyncVal _ vl _ => vl
-        end.
+    Global Arguments SyncVal {A}.
+    Global Arguments NonSyncVal {A}.
 
-      Definition projRight {σ} (rv : RelVal σ) : Val σ :=
-        match rv with
-        | SyncVal _ v => v
-        | NonSyncVal _ _ vr => vr
-        end.
+    Definition projLeftRV {A} (rv : RV A) : A :=
+      match rv with
+      | SyncVal v => v
+      | NonSyncVal vl _ => vl
+      end.
 
-      Definition liftBinOp {σ1 σ2 σ3} (f : Val σ1 -> Val σ2 -> Val σ3) (rv1 : RelVal σ1) (rv2 : RelVal σ2) : RelVal σ3 :=
-        match (rv1 , rv2) with
-        | (SyncVal _ v1 , SyncVal _ v2) => SyncVal _ (f v1 v2)
-        | (_ , _) => NonSyncVal _ (f (projLeft rv1) (projLeft rv2)) (f (projRight rv1) (projRight rv2))
-        end.
+    Definition projRightRV {A} (rv : RV A) : A :=
+      match rv with
+      | SyncVal v => v
+      | NonSyncVal _ vr => vr
+      end.
 
-      Definition liftUnOp {σ1 σ2} (f : Val σ1 -> Val σ2) (rv : RelVal σ1) : RelVal σ2 :=
-        match rv with
-        | (SyncVal _ v) => SyncVal _ (f v)
-        | (NonSyncVal _ vl vr) => NonSyncVal _ (f vl) (f vr)
-        end.
+    Definition liftUnOpRV {A B} (f : A -> B) (rv : RV A) : RV B :=
+      match rv with
+      | (SyncVal v) => SyncVal (f v)
+      | (NonSyncVal vl vr) => NonSyncVal (f vl) (f vr)
+      end.
 
-      Definition isSyncVal {σ} (v : RelVal σ) : Datatypes.bool :=
-        match v with
-        | SyncVal _ _ => true
-        | NonSyncVal _ _ _ => false
-        end.
+    Definition liftBinOpRV {A B C} (f : A -> B -> C) (rv1 : RV A) (rv2 : RV B) : RV C :=
+      match (rv1 , rv2) with
+      | (SyncVal v1 , SyncVal v2) => SyncVal (f v1 v2)
+      | (_ , _) => NonSyncVal (f (projLeftRV rv1) (projLeftRV rv2)) (f (projRightRV rv1) (projRightRV rv2))
+      end.
+    
+    Definition rv_equiv (rv1 : RV Prop) (rv2 : RV Prop) : RV Prop :=
+      match rv1, rv2 with
+      | SyncVal p, SyncVal q => SyncVal (p <-> q)
+      | SyncVal p, NonSyncVal q1 q2 => NonSyncVal (p <-> q1) (p <-> q2)
+      | NonSyncVal p1 p2, SyncVal q => NonSyncVal (p1 <-> q) (p2 <-> q)
+      | NonSyncVal p1 p2, NonSyncVal q1 q2 => NonSyncVal (p1 <-> q1) (p2 <-> q2)
+      end.
 
-      Definition isSyncValProp {σ} (v : RelVal σ) : Prop :=
-        match v with
-        | SyncVal _ _ => True
-        | NonSyncVal _ _ _ => False
-        end.
-      
+    Definition rv_impl (rv1 : RV Prop) (rv2 : RV Prop) : RV Prop :=
+      match rv1, rv2 with
+      | SyncVal p1, SyncVal p2 => SyncVal (p1 -> p2)
+      | SyncVal p, NonSyncVal q1 q2 => NonSyncVal (p -> q1) (p -> q2)
+      | NonSyncVal p1 p2, SyncVal q => NonSyncVal (p1 -> q) (p2 -> q)
+      | NonSyncVal p1 p2, NonSyncVal q1 q2 => NonSyncVal (p1 -> q1) (p2 -> q2)
+      end.
 
-      Definition relValPairIsPairRelVal {σ1 σ2} (rv : RelVal (prod σ1 σ2)) : RelVal σ1 * RelVal σ2 :=
-        match rv with
-        | SyncVal _ (a , b) => (SyncVal _ a, SyncVal _ b)
-        | NonSyncVal _ (a1, b1) (a2, b2) => (NonSyncVal _ a1 a2, NonSyncVal _ b1 b2)
-        end.
+    Definition rv_bientails (rv1 : RV Prop) (rv2 : RV Prop) : Prop :=
+      match rv1, rv2 with
+      | SyncVal p, SyncVal q => p <-> q
+      | SyncVal p, NonSyncVal q1 q2 => (p <-> q1) /\ (p <-> q2)
+      | NonSyncVal p1 p2, SyncVal q => (p1 <-> q) /\ (p2 <-> q)
+      | NonSyncVal p1 p2, NonSyncVal q1 q2 => (p1 <-> q1) /\ (p2 <-> q2)
+      end.
 
-      Definition pairRelValIsRelValPair {σ1 σ2} (rv_pair : RelVal σ1 * RelVal σ2) : RelVal (prod σ1 σ2) :=
+    Definition rv_entails (rv1 : RV Prop) (rv2 : RV Prop) : Prop :=
+      match rv1, rv2 with
+      | SyncVal p, SyncVal q => p -> q
+      | SyncVal p, NonSyncVal q1 q2 => (p -> q1) /\ (p -> q2)
+      | NonSyncVal p1 p2, SyncVal q => (p1 -> q) /\ (p2 -> q)
+      | NonSyncVal p1 p2, NonSyncVal q1 q2 => (p1 -> q1) /\ (p2 -> q2)
+      end.
+
+    (* Definition rv_equiv_is_iff (rv1 : RV Prop) (rv2 : RV Prop) : rv_equiv rv1 rv2 <-> (rv_impl rv1 rv2 /\ rv_impl rv2 rv1). *)
+    (* Proof. *)
+    (*   destruct rv1; destruct rv2; cbn; tauto. *)
+    (* Qed. *)
+
+    Definition rv_neg (rv : RV Prop) : RV Prop :=
+      match rv with
+      | SyncVal p1 => SyncVal (~ p1)
+      | NonSyncVal p1 p2 => NonSyncVal (~ p1) (~ p2)
+      end.
+
+    Definition rv_entails_refl : Reflexive (rv_entails).
+    Proof. unfold Reflexive, rv_entails. intros.
+           destruct x; cbn; auto.
+    Qed.
+
+    Definition rv_entails_trans : Transitive (rv_entails).
+    Proof.
+      unfold Transitive, rv_entails.
+      intros.
+      destruct x; destruct y; destruct z; cbn in *; eauto; try contradiction; try tauto.
+    Qed.
+
+    #[export] Instance preorder_entails : PreOrder (rv_entails).
+    Proof. split; auto using rv_entails_refl, rv_entails_trans. Qed.
+
+    #[export] Instance equivalence_bientails : Equivalence (rv_bientails).
+    Proof.
+      unfold rv_bientails. constructor.
+      - unfold Reflexive. intros. destruct x; cbn; auto.
+      - unfold Symmetric. intros. destruct x; destruct y; cbn in *; tauto.
+      - unfold Transitive. intros.
+        destruct x; destruct y; destruct z; cbn in *; eauto; try contradiction; tauto.
+    Qed.
+
+    #[export] Instance subrelation_bientails_entails :
+      subrelation (rv_bientails) (rv_entails).
+    Proof. intros x y xy.
+           destruct x; destruct y; cbn in *; try apply xy;
+             tauto.
+    Qed.
+
+    #[export,program] Instance proper_rv_bientails (rv1 rv2 : RV Prop) :
+      Proper (rv_bientails ==> rv_bientails ==> iff) (rv_bientails).
+    Next Obligation.
+      intros rv1 rv2.
+      intros p1 p2 Rp q1 q2 Rq. 
+      unfold rv_bientails in *.
+      destruct p1; destruct p2; destruct q1; destruct q2; cbn; tauto.
+    Qed.
+
+    #[export,program] Instance proper_rv_equiv (rv1 rv2 : RV Prop) :
+       Proper (rv_bientails ==> rv_bientails ==> rv_bientails) (rv_equiv).
+    Next Obligation.
+      intros rv1 rv2.
+      intros p1 p2 Rp q1 q2 Rq. 
+      unfold rv_bientails in *. unfold rv_equiv.
+      destruct p1; destruct p2; destruct q1; destruct q2; cbn; tauto.
+    Qed.
+
+    #[export,program] Instance proper_rv_entails (rv1 rv2 : RV Prop) :
+      Proper (rv_bientails ==> rv_bientails ==> iff) (rv_entails).
+    Next Obligation.
+      intros rv1 rv2.
+      intros p1 p2 Rp q1 q2 Rq. 
+      unfold rv_bientails in *.
+      destruct p1; destruct p2; destruct q1; destruct q2; cbn; tauto.
+    Qed.
+
+    #[export,program] Instance proper_rv_impl (rv1 rv2 : RV Prop) :
+      Proper (rv_bientails ==> rv_bientails ==> rv_bientails) (rv_impl).
+    Next Obligation.
+      intros rv1 rv2.
+      intros p1 p2 Rp q1 q2 Rq. 
+      unfold rv_bientails in *.
+      destruct p1; destruct p2; destruct q1; destruct q2; cbn; tauto.
+    Qed.
+
+    #[export,program] Instance proper_rv_impl_mono' (rv1 rv2 : RV Prop) :
+      Proper (rv_entails --> rv_entails ==> rv_entails) (rv_impl).
+    Next Obligation.
+      intros rv1 rv2.
+      intros p1 p2 Rp q1 q2 Rq. 
+      unfold rv_entails in *. cbn in *.
+      destruct p1; destruct p2; destruct q1; destruct q2; cbn; tauto.
+    Qed.
+
+    #[export,program] Instance proper_rv_impl_flip_mono' (rv1 rv2 : RV Prop) :
+      Proper (rv_entails ==> flip(rv_entails) ==> flip(rv_entails)) (rv_impl).
+    Next Obligation.
+      intros rv1 rv2.
+      intros p1 p2 Rp q1 q2 Rq. 
+      unfold rv_entails in *. cbn in *.
+      destruct p1; destruct p2; destruct q1; destruct q2; cbn; tauto.
+    Qed.
+
+
+    Context {TDC : TypeDeclKit}.
+    Context {TDN : TypeDenoteKit TDC}.
+    
+    Fixpoint RelVal (σ : Ty) : Set :=
+      match σ with
+      | int => RV (Val int)
+      | bool => RV (Val bool)
+      | string => RV (Val string)
+      | list σ' => Datatypes.list (RelVal σ')
+      | prod σ1 σ2 => RelVal σ1 * RelVal σ2
+      (* | sum σ1 σ2 => RV (RelVal σ1 + RelVal σ2) *)
+      | unit => Datatypes.unit
+      | bvec n => RV (Val (bvec n))
+      end%type.
+
+    Fixpoint valToRelVal {σ} : Val σ -> RelVal σ :=
+      match σ return Val σ -> RelVal σ with
+      | int => fun v => SyncVal v
+      | bool => fun v => SyncVal v
+      | string => fun v => SyncVal v
+      | list σ' => fun v => List.map valToRelVal v
+      | prod σ1 σ2 => fun v => (valToRelVal (fst v), valToRelVal (snd v))
+      (* | sum σ1 σ2 => fun v => match v with *)
+      (*                         | inl v => SyncVal (inl (valToRelVal v)) *)
+      (*                         | inr v => SyncVal (inr (valToRelVal v)) *)
+      (*                         end *)
+      | unit => fun v => tt
+      | bvec n => fun v => SyncVal v
+      end%type.
+
+    Fixpoint map {σ} : (forall σ, RV (Val σ) -> Val σ) -> RelVal σ -> Val σ :=
+      match σ return (forall σ, RV (Val σ) -> Val σ) -> RelVal σ -> Val σ with
+      | int => fun f rv => f _ rv
+      | bool => fun f rv => f _ rv
+      | string => fun f rv => f _ rv
+      | list σ' => fun f rv => List.map (map f) rv
+      | prod σ1 σ2 => fun f rv => (map f (fst rv), map f (snd rv))
+      (* | sum σ1 σ2 => fun f rv => f _ rv *)
+      | unit => fun f rv => tt
+      | bvec n => fun f rv => f _ rv
+      end%type.
+
+    Definition projLeft {σ} (rv : RelVal σ) : Val σ :=
+      map (fun σ => @projLeftRV (Val σ)) rv.
+
+    Definition projRight {σ} (rv : RelVal σ) : Val σ :=
+      map (fun σ => @projRightRV (Val σ)) rv.
+
+    Fixpoint listOfRVToRVOfList {A} (rv_list : (Datatypes.list (RV A))) : RV (Datatypes.list A) :=
+      match rv_list with
+      | nil => SyncVal nil
+      | (x :: l)%list => liftBinOpRV cons x (listOfRVToRVOfList l)
+      end.
+
+    Definition RVOfPairToPairOfRV {σ1 σ2} (rv : RV (σ1 * σ2)) : RV σ1 * RV σ2 :=
+      match rv with
+      | SyncVal (a , b) => (SyncVal a, SyncVal b)
+      | NonSyncVal (a1, b1) (a2, b2) => (NonSyncVal a1 a2, NonSyncVal b1 b2)
+      end.
+
+      Definition pairOfRVToRVOfPair {σ1 σ2} (rv_pair : RV σ1 * RV σ2) : RV (σ1 * σ2) :=
         match rv_pair with
-        | (SyncVal _ v1 , SyncVal _ v2) => SyncVal (prod σ1 σ2) (v1, v2)
-        | (rv1, rv2) => NonSyncVal (prod σ1 σ2) (projLeft rv1, projLeft rv2) (projRight rv1, projRight rv2)
+        | (SyncVal v1 , SyncVal v2) => SyncVal (v1, v2)
+        | (rv1, rv2) => NonSyncVal (projLeftRV rv1, projLeftRV rv2) (projRightRV rv1, projRightRV rv2)
         end.
 
-      Fixpoint listRelValIsRelValList {σ} (rv_list : (Datatypes.list (RelVal σ))) : RelVal (list σ) :=
-        match rv_list with
-        | nil => SyncVal (list _) nil
-        | (x :: l)%list => liftBinOp (σ2 := list _) (σ3 := list _) cons x (listRelValIsRelValList l)
-        end.
+    Fixpoint relValToRV {σ} : RelVal σ -> RV (Val σ) :=
+      match σ return RelVal σ -> RV (Val σ) with
+      | int => id
+      | bool => id
+      | string => id
+      | list σ' => fun rv => listOfRVToRVOfList (List.map relValToRV rv)
+      | prod σ1 σ2 => fun rv => pairOfRVToRVOfPair (relValToRV (fst rv), relValToRV (snd rv))
+      (* | sum σ1 σ2 => id *)
+      | unit => fun rv => SyncVal tt
+      | bvec n => id
+      end%type.
 
-      Fixpoint vecRelValIsRelValVec {n} (rv_vec : Vector.t (RelVal bool) n) : RelVal (ty.bvec n) :=
-        match rv_vec with
-        | Vector.nil => SyncVal (bvec _) bv.nil
-        | Vector.cons x l => liftBinOp (σ1 := bool) (σ2 := bvec _) (σ3 := bvec _) (bv.cons (n := _)) x (vecRelValIsRelValVec l)
-        end.
+    Lemma valToRelValToRVIsSyncVal {σ} (v : Val σ) : relValToRV (valToRelVal v) = SyncVal v.
+    Proof.
+      induction σ; try reflexivity.
+      - cbn. induction v.
+        + auto.
+        + cbn. rewrite IHv. rewrite IHσ. auto.
+      - destruct v. cbn. rewrite IHσ1, IHσ2. auto.
+      - destruct v. auto.
+    Qed.
 
-      Fixpoint sumRelValIsRelValSum {σ1 σ2} (rv_sum : RelVal σ1 + RelVal σ2) : RelVal (sum σ1 σ2) :=
-        match rv_sum with
-        | inl rv => match rv with
-                    | SyncVal _ v => SyncVal (sum _ _) (inl v)
-                    | NonSyncVal _ v1 v2 => NonSyncVal (sum _ _) (inl v1) (inl v2)
-                    end
-        | inr rv => match rv with
-                    | SyncVal _ v => SyncVal (sum _ _) (inr v)
-                    | NonSyncVal _ v1 v2 => NonSyncVal (sum _ _) (inr v1) (inr v2)
-                    end
-        end.
+    (* This function "and"s the result in case of lists and pairs and unit is automatically true *)
+    (*  TODO: I am not a 100% sure that this method isn't more misleading than helpful. *)
+    Fixpoint liftBoolFuncRelValAnd {σ} (f : forall σ', RV σ' -> Datatypes.bool) :
+      RelVal σ -> Datatypes.bool :=
+      match σ return RelVal σ -> Datatypes.bool with
+      | int => fun rv => f _ rv
+      | bool => fun rv => f _ rv
+      | string => fun rv => f _ rv
+      | list σ' => fun rv => fold_right andb true (List.map (liftBoolFuncRelValAnd f) rv)
+      | prod σ1 σ2 => fun rv => liftBoolFuncRelValAnd f (fst rv) && liftBoolFuncRelValAnd f (snd rv)
+      (* | sum σ1 σ2 => fun rv => f _ rv *)
+      | unit => fun rv => true
+      | bvec n => fun rv => f _ rv
+      end%type.
 
-      Fixpoint liftNamedEnv {varkit b} (a : @NamedEnv (@Variables.PVar varkit) Ty Val b) : @NamedEnv (@Variables.PVar varkit) Ty RelVal b :=
-        match a with
-        | env.nil => env.nil
-        | env.snoc e x db => env.snoc (liftNamedEnv e) x (SyncVal _ db)
-        end.
+    Fixpoint liftPropFuncRelValAnd {σ} (f : forall σ', RV σ' -> Prop) :
+      RelVal σ -> Prop :=
+      match σ return RelVal σ -> Prop with
+      | int => fun rv => f _ rv
+      | bool => fun rv => f _ rv
+      | string => fun rv => f _ rv
+      | list σ' => fun rv => fold_right and True (List.map (liftPropFuncRelValAnd f) rv)
+      | prod σ1 σ2 => fun rv => liftPropFuncRelValAnd f (fst rv) /\ liftPropFuncRelValAnd f (snd rv)
+      (* | sum σ1 σ2 => fun rv => f _ rv *)
+      | unit => fun rv => True
+      | bvec n => fun rv => f _ rv
+      end%type.
 
-      Fixpoint NamedEnvValToRelVal {N Γ} (nenv1 : @NamedEnv N Ty Val Γ) : NamedEnv Val Γ -> NamedEnv RelVal Γ :=
-        match nenv1 with
-          | env.nil => fun nenv2 => env.nil
-          | env.snoc nenv1' b1 db1 =>
-              fun nenv2 =>
-                match env.view nenv2 with
-                  env.isSnoc nenv2' db2 => env.snoc (NamedEnvValToRelVal nenv1' nenv2') b1 (NonSyncVal (type b1) db1 db2)
-                end
-          end.
+    Definition isSyncValRV {σ} (rv : RV σ) : Datatypes.bool :=
+      match rv with
+      | SyncVal _ => true
+      | NonSyncVal _ _ => false
+      end.
+
+    Definition isSyncVal {σ} : RelVal σ -> Datatypes.bool :=
+      liftBoolFuncRelValAnd (@isSyncValRV).
+
+    Definition isSyncValPropRV {σ} (v : RV σ) : Prop :=
+      match v with
+      | SyncVal _ => True
+      | NonSyncVal _ _ => False
+      end.
+
+    Definition isSyncValProp {σ} : RelVal σ -> Prop :=
+      liftPropFuncRelValAnd (@isSyncValPropRV).
       
 
-      Fixpoint mapSyncValNamedEnv {X Σ} (ı : NamedEnv (X := X) Val Σ) : NamedEnv (X := X) RelVal Σ :=
-        match ı with
-        | env.nil => env.nil
-        | env.snoc E db v => env.snoc (mapSyncValNamedEnv E) db (SyncVal (type db) v)
+      Fixpoint vecOfRVToRVOfVec {n} (rv_vec : Vector.t (RV (Val bool)) n) : RV (Val (ty.bvec n)) :=
+        match rv_vec with
+        | Vector.nil => SyncVal bv.nil
+        | Vector.cons x l => liftBinOpRV (A := Val bool) (B := Val (bvec _)) (C := Val (bvec _)) (bv.cons (n := _)) x (vecOfRVToRVOfVec l)
         end.
 
-      Fixpoint allSync {X Σ} (ı : NamedEnv (X := X) RelVal Σ) : Prop :=
-        match ı with
-        | env.nil => True
-        | env.snoc E db v => match v with
-                             | SyncVal _ _ => allSync E
-                             | _ => False
-                             end
-        end.
+      (* Fixpoint sumRelValIsRelValSum {σ1 σ2} (rv_sum : RelVal σ1 + RelVal σ2) : RelVal (sum σ1 σ2) := *)
+      (*   match rv_sum with *)
+      (*   | inl rv => match rv with *)
+      (*               | SyncVal _ v => SyncVal (sum _ _) (inl v) *)
+      (*               | NonSyncVal _ v1 v2 => NonSyncVal (sum _ _) (inl v1) (inl v2) *)
+      (*               end *)
+      (*   | inr rv => match rv with *)
+      (*               | SyncVal _ v => SyncVal (sum _ _) (inr v) *)
+      (*               | NonSyncVal _ v1 v2 => NonSyncVal (sum _ _) (inr v1) (inr v2) *)
+      (*               end *)
+      (*   end. *)
 
-      Fixpoint allNonSync {X Σ} (ı : NamedEnv (X := X) RelVal Σ) : Prop :=
-        match ı with
-        | env.nil => True
-        | env.snoc E db v => match v with
-                             | NonSyncVal _ _ _ => allNonSync E
-                             | _ => False
-                             end
-        end.
+      (* Fixpoint liftNamedEnv {varkit b} (a : @NamedEnv (@Variables.PVar varkit) Ty Val b) : @NamedEnv (@Variables.PVar varkit) Ty RelVal b := *)
+      (*   match a with *)
+      (*   | env.nil => env.nil *)
+      (*   | env.snoc e x db => env.snoc (liftNamedEnv e) x (SyncVal _ db) *)
+      (*   end. *)
 
-      Fixpoint namedEnvRel_to_nonsyncval {X Σ} (nenv : NamedEnv (X := X) RelVal Σ) : NamedEnv (X := X) RelVal Σ :=
-        match nenv with
-        | env.nil => env.nil
-        | env.snoc E db rv =>
-            match rv with
-            | NonSyncVal _ _ _ => env.snoc (namedEnvRel_to_nonsyncval E) db rv
-            | SyncVal _ v => env.snoc (namedEnvRel_to_nonsyncval E) db (NonSyncVal _ v v)
-            end
-        end.
+      (* Fixpoint NamedEnvValToRelVal {N Γ} (nenv1 : @NamedEnv N Ty Val Γ) : NamedEnv Val Γ -> NamedEnv RelVal Γ := *)
+      (*   match nenv1 with *)
+      (*   | env.nil => fun nenv2 => env.nil *)
+      (*   | env.snoc nenv1' b1 db1 => *)
+      (*       fun nenv2 => *)
+      (*         match env.view nenv2 with *)
+      (*           env.isSnoc nenv2' db2 => env.snoc (NamedEnvValToRelVal nenv1' nenv2') b1 (NonSyncVal (type b1) db1 db2) *)
+      (*         end *)
+      (*   end. *)
+      
+
+      (* Fixpoint mapSyncValNamedEnv {X Σ} (ı : NamedEnv (X := X) Val Σ) : NamedEnv (X := X) RelVal Σ := *)
+      (*   match ı with *)
+      (*   | env.nil => env.nil *)
+      (*   | env.snoc E db v => env.snoc (mapSyncValNamedEnv E) db (SyncVal (type db) v) *)
+      (*   end. *)
+
+      (* Fixpoint allSync {X Σ} (ı : NamedEnv (X := X) RelVal Σ) : Prop := *)
+      (*   match ı with *)
+      (*   | env.nil => True *)
+      (*   | env.snoc E db v => match v with *)
+      (*                        | SyncVal _ _ => allSync E *)
+      (*                        | _ => False *)
+      (*                        end *)
+      (*   end. *)
+
+      (* Fixpoint allNonSync {X Σ} (ı : NamedEnv (X := X) RelVal Σ) : Prop := *)
+      (*   match ı with *)
+      (*   | env.nil => True *)
+      (*   | env.snoc E db v => match v with *)
+      (*                        | NonSyncVal _ _ _ => allNonSync E *)
+      (*                        | _ => False *)
+      (*                        end *)
+      (*   end. *)
+
+      (* Fixpoint namedEnvRel_to_nonsyncval {X Σ} (nenv : NamedEnv (X := X) RelVal Σ) : NamedEnv (X := X) RelVal Σ := *)
+      (*   match nenv with *)
+      (*   | env.nil => env.nil *)
+      (*   | env.snoc E db rv => *)
+      (*       match rv with *)
+      (*       | NonSyncVal _ _ _ => env.snoc (namedEnvRel_to_nonsyncval E) db rv *)
+      (*       | SyncVal _ v => env.snoc (namedEnvRel_to_nonsyncval E) db (NonSyncVal _ v v) *)
+      (*       end *)
+      (*   end. *)
+
+    Unset Universe Polymorphism.
 
   End WithTypeDenote.
 
@@ -350,7 +593,7 @@ Module ty.
         | string     , string     => left eq_refl
         | list σ     , list τ     => f_equal_dec list noConfusion_inv (ty_eqdec σ τ)
         | prod σ1 σ2 , prod τ1 τ2 => f_equal2_dec prod noConfusion_inv (ty_eqdec σ1 τ1) (ty_eqdec σ2 τ2)
-        | sum σ1 σ2  , sum τ1 τ2  => f_equal2_dec sum noConfusion_inv (ty_eqdec σ1 τ1) (ty_eqdec σ2 τ2)
+        (* | sum σ1 σ2  , sum τ1 τ2  => f_equal2_dec sum noConfusion_inv (ty_eqdec σ1 τ1) (ty_eqdec σ2 τ2) *)
         | unit       , unit       => left eq_refl
 (*        | enum E1    , enum E2    => f_equal_dec enum noConfusion_inv (eq_dec E1 E2) *)
         | bvec n1    , bvec n2    => f_equal_dec bvec noConfusion_inv (eq_dec n1 n2)
@@ -370,7 +613,7 @@ Module ty.
         | string   => eq_dec (A := String.string)
         | list σ   => eq_dec (A := Datatypes.list (Val σ))
         | prod σ τ => eq_dec (A := Datatypes.prod (Val σ) (Val τ))
-        | sum σ τ  => eq_dec (A := Datatypes.sum (Val σ) (Val τ))
+        (* | sum σ τ  => eq_dec (A := Datatypes.sum (Val σ) (Val τ)) *)
         | unit     => eq_dec (A := Datatypes.unit)
  (*       | enum E   => eq_dec (A := enumt E) *)
         | bvec n   => eq_dec (A := bv n)
@@ -386,45 +629,59 @@ Module ty.
         | record R => eq_dec (A := recordt R) *)
         end.
 
-    Lemma helper {τ} {x y1 y2 : Val τ} : NonSyncVal τ y1 y2 = SyncVal τ x -> False.
+    Lemma helper {A} {x y1 y2 : A} : NonSyncVal y1 y2 = SyncVal x -> False.
     Proof.
       congruence.
       Show Proof.
     Qed.      
 
 
-    #[export] Instance RelVal_eq_dec : forall σ, EqDec (RelVal σ) :=
+    #[export] Instance RV_eq_dec : forall σ, EqDec (RV (Val σ)) :=
       fun σ x y => match x , y with
-                   | SyncVal _ x , SyncVal _ y => match eq_dec x y with
-                                                  | left eq => left (f_equal (SyncVal _) eq)
-                                                  | right neq => right (fun p : SyncVal _ _ = SyncVal _ _ => neq (f_equal projLeft p))
+                   | SyncVal x , SyncVal y => match eq_dec x y with
+                                                  | left eq => left (f_equal SyncVal eq)
+                                                  | right neq => right (fun p : SyncVal _ = SyncVal _ => neq (f_equal projLeftRV p))
                                                   end
-                   | NonSyncVal _ x1 x2 , NonSyncVal _ y1 y2 =>
+                   | NonSyncVal x1 x2 , NonSyncVal y1 y2 =>
                        match eq_dec x1 y1 , eq_dec x2 y2 with
-                       | left eq1 , left eq2 => left (f_equal2 (NonSyncVal _) eq1 eq2)
-                       | right neq1, _ => right (fun p : NonSyncVal _ _ _ = NonSyncVal _ _ _ => neq1 (f_equal projLeft p))
-                       | _, right neq2 => right (fun p : NonSyncVal _ _ _ = NonSyncVal _ _ _ => neq2 (f_equal projRight p))
+                       | left eq1 , left eq2 => left (f_equal2 NonSyncVal eq1 eq2)
+                       | right neq1, _ => right (fun p : NonSyncVal _ _ = NonSyncVal _ _ => neq1 (f_equal projLeftRV p))
+                       | _, right neq2 => right (fun p : NonSyncVal _ _ = NonSyncVal _ _ => neq2 (f_equal projRightRV p))
                        end
-                   | SyncVal _ x , NonSyncVal _ y1 y2 =>
+                   | SyncVal x , NonSyncVal y1 y2 =>
                        right (fun Heq =>
                        let H0 : False :=
-                         eq_ind (SyncVal _ x)
-                           (fun e : RelVal _ => match e with
-                                                | SyncVal _ _ => True
-                                                | NonSyncVal _ _ _ => False
-                                                end) I (NonSyncVal _ y1 y2) Heq in
+                         eq_ind (SyncVal x)
+                           (fun e : RV _ => match e with
+                                                | SyncVal _ => True
+                                                | NonSyncVal _ _ => False
+                                                end) I (NonSyncVal y1 y2) Heq in
                        False_ind False H0)
-                   | NonSyncVal _ x1 x2 , SyncVal _ y =>
+                   | NonSyncVal x1 x2 , SyncVal y =>
                        right (fun Heq =>
                        let H0 : False :=
-                         eq_ind (NonSyncVal _ x1 x2)
-                           (fun e : RelVal _ =>
+                         eq_ind (NonSyncVal x1 x2)
+                           (fun e : RV _ =>
                               match e with
-                              | SyncVal _ _ => False
-                              | NonSyncVal _ _ _ => True
-                              end) I (SyncVal _ y) Heq in
+                              | SyncVal _ => False
+                              | NonSyncVal _ _ => True
+                              end) I (SyncVal y) Heq in
                        False_ind False H0)
                    end.
+
+        #[export] Instance RelVal_eq_dec : forall σ, EqDec (RelVal σ) :=
+      fix eqd σ :=
+        match σ return EqDec (RelVal σ) with
+        | int      => RV_eq_dec _
+        | bool     => RV_eq_dec _
+        | string   => RV_eq_dec _
+        | list σ   => eq_dec (A := Datatypes.list (RelVal σ))
+        | prod σ τ => eq_dec (A := Datatypes.prod (RelVal σ) (RelVal τ))
+        (* | sum σ τ  => RV_eq_dec _ *)
+        | unit     => eq_dec (A := Datatypes.unit)
+        | bvec n   => RV_eq_dec _
+        end.
+
 
  (*   Lemma unionv_fold_inj {U} (v1 v2 : {K : unionk U & Val (unionk_ty U K)}) :
       unionv_fold U v1 = unionv_fold U v2 <-> v1 = v2.
@@ -469,7 +726,7 @@ Module ty.
   #[global] Arguments string {TK}.
   #[global] Arguments list {TK} σ.
   #[global] Arguments prod {TK} σ τ.
-  #[global] Arguments sum {TK} σ τ.
+  (* #[global] Arguments sum {TK} σ τ. *)
   #[global] Arguments unit {TK}.
   (*  #[global] Arguments enum {TK} E. *)
   #[global] Arguments bvec {TK} n%_nat_scope.
