theories/Syntax/UnOps.v
@@ -50,8 +50,8 @@ Module uop.
     Context {TDC : TypeDeclKit}.
 
     Variant UnOp : Ty -> Ty -> Set :=
-    | inl {σ1 σ2 : Ty}  : UnOp σ1 (sum σ1 σ2)
-    | inr {σ1 σ2 : Ty}  : UnOp σ2 (sum σ1 σ2)
+    (* | inl {σ1 σ2 : Ty}  : UnOp σ1 (sum σ1 σ2) *)
+    (* | inr {σ1 σ2 : Ty}  : UnOp σ2 (sum σ1 σ2) *)
     | neg               : UnOp int int
     | not               : UnOp bool bool
     | sext {m n} {p : IsTrue (m <=? n)} : UnOp (bvec m) (bvec n)
@@ -89,8 +89,8 @@ Module uop.
     #[derive(equations=no)] Equations tel_eq_dec {σ1 σ2 τ : Ty}
       (op1 : UnOp σ1 τ) (op2 : UnOp σ2 τ) :
       dec_eq (A := Tel τ) (sigmaI _ σ1 op1) (sigmaI _ σ2 op2) :=
-    | inl                              | inl => left eq_refl
-    | inr                              | inr => left eq_refl
+    (* | inl                              | inl => left eq_refl *)
+    (* | inr                              | inr => left eq_refl *)
     | neg                              | neg => left eq_refl
     | not                              | not => left eq_refl
     | @sext _ m1 ?(n) p1               | @sext _ m2 n p2 with eq_dec m1 m2 => {
@@ -134,8 +134,8 @@ Module uop.
 
     Definition eval {σ1 σ2 : Ty} (op : UnOp σ1 σ2) : Val σ1 -> Val σ2 :=
       match op in UnOp σ1 σ2 return Val σ1 -> Val σ2 with
-      | inl                 => Datatypes.inl
-      | inr                 => Datatypes.inr
+      (* | inl                 => Datatypes.inl *)
+      (* | inr                 => Datatypes.inr *)
       | neg                 => Z.opp
       | not                 => negb
       | sext                => fun v => bv.sext v
@@ -147,6 +147,23 @@ Module uop.
       | vector_subrange s l => bv.vector_subrange s l
       | bvnot               => bv.not
       | negate              => bv.negate
+      end.
+
+    Definition evalRel {σ1 σ2 : Ty} (op : UnOp σ1 σ2) : RelVal σ1 -> RelVal σ2 :=
+      match op in UnOp σ1 σ2 return RelVal σ1 -> RelVal σ2 with
+      (* | inl                 => liftUnOpRV Datatypes.inl *)
+      (* | inr                 => Datatypes.inr *)
+      | neg                 => liftUnOpRV Z.opp
+      | not                 => liftUnOpRV negb
+      | sext                => liftUnOpRV (fun v => bv.sext v)
+      | zext                => liftUnOpRV (fun v => bv.zext v)
+      | get_slice_int       => liftUnOpRV bv.of_Z
+      | signed              => liftUnOpRV (fun v => bv.signed v)
+      | unsigned            => liftUnOpRV (fun v => bv.unsigned v)
+      | truncate m          => liftUnOpRV (fun v => bv.truncate m v)
+      | vector_subrange s l => liftUnOpRV (bv.vector_subrange s l)
+      | bvnot               => liftUnOpRV bv.not
+      | negate              => liftUnOpRV bv.negate
       end.
 
   End WithTypeDef.
