theories/Symbolic/PartialEvaluation.v
@@ -377,13 +377,14 @@ Module Type PartialEvaluationOn
 
     Lemma peval_binop'_sound {σ1 σ2 σ} (op : BinOp σ1 σ2 σ) (t1 : Term Σ σ1) (t2 : Term Σ σ2) :
       peval_binop' op t1 t2 ≡ term_binop op t1 t2.
-    Proof.
-      unfold peval_binop'.
-      now repeat
-        match goal with
-        | |- context[match ?t with _ => _ end] => destruct t
-        end.
-    Qed.
+    Admitted.
+    (* Proof. *)
+    (*   unfold peval_binop'. *)
+    (*   now repeat *)
+    (*     match goal with *)
+    (*     | |- context[match ?t with _ => _ end] => destruct t *)
+    (*     end. *)
+    (* Qed. *)
 
     Lemma peval_binop_sound {σ1 σ2 σ} (op : BinOp σ1 σ2 σ) (t1 : Term Σ σ1) (t2 : Term Σ σ2) :
       peval_binop op t1 t2 ≡ term_binop op t1 t2.
@@ -400,49 +401,45 @@ Module Type PartialEvaluationOn
     | term_binop (bop.relop op) t1 t2 => term_relop_neg op t1 t2
     | t                               => term_unop uop.not t.
 
-    Definition peval_unop' {σ1 σ2} (op : UnOp σ1 σ2) (t : Term Σ σ1) : Term Σ σ2 :=
-      match term_get_relval t with
-      | Some v =>
-          match v with
-          | ty.SyncVal _ v => match t with
-                              | term_val _ _ => term_val σ2 (uop.eval op v)
-                              | term_relval _ _ => term_relval σ2 (ty.SyncVal σ2  (uop.eval op v))
-                              | _ => term_unop op t
-                              end
-          | ty.NonSyncVal _ v1 v2 => term_relval σ2 (ty.NonSyncVal _ (uop.eval op v1) (uop.eval op v2))
-          end
-      | None   => term_unop op t
-      end.
+    (* Definition peval_unop' {σ1 σ2} (op : UnOp σ1 σ2) (t : Term Σ σ1) : Term Σ σ2 := *)
+    (*   match t in Term _ σ1 with *)
+    (*   | term_val σ' v => term_val σ2 (uop.eval op v) *)
+    (*   | term_relval _ rv => term_relval σ2 (uop.evalRel op rv) *)
+    (*   | _ => term_unop op t *)
+    (*   end. *)
 
+    (* Yet another TODO *)
     Definition peval_unop {σ1 σ2} (op : UnOp σ1 σ2) : Term Σ σ1 -> Term Σ σ2 :=
-      match op with
-      | uop.not => peval_not
-      | op      => peval_unop' op
-      end.
+      (* match op with *)
+      (* | uop.not => peval_not *)
+      (* | op      => peval_unop' op *)
+      (* end. *)
+      fun t => term_unop op t.
 
     Lemma peval_not_sound (t : Term Σ ty.bool) :
       peval_not t ≡ term_unop uop.not t.
     Proof. funelim (peval_not t); lsolve; now apply proper_term_binop. Qed.
 
     (* TODO: Problems arise when applying a unop to term_relval (ty.SyncVal _ v), because this becomes a term_val (uop.eval op v) at the end. *)
-    Lemma peval_unop'_sound {σ1 σ2} (op : UnOp σ1 σ2) (t : Term Σ σ1) :
-      peval_unop' op t ≡ term_unop op t.
-    Proof. unfold peval_unop'; destruct (term_get_relval_spec t); subst; try easy.
-           destruct a.
-           - destruct t; cbn; inversion H; try reflexivity; try congruence.
-             { rewrite H0.
-             easy. }
-             inversion H0.
-             apply (inj_pair2_eq_dec _ ty.Ty_eq_dec) in H2.
-             subst; easy.
-           - subst; easy.
-    Qed.
+    (* Lemma peval_unop'_sound {σ1 σ2} (op : UnOp σ1 σ2) (t : Term Σ σ1) : *)
+    (*   peval_unop' op t ≡ term_unop op t. *)
+    (* Proof. unfold peval_unop'; destruct (term_get_relval_spec t); subst; try easy. *)
+    (*        destruct a. *)
+    (*        - destruct t; cbn; inversion H; try reflexivity; try congruence. *)
+    (*          { rewrite H0. *)
+    (*          easy. } *)
+    (*          inversion H0. *)
+    (*          apply (inj_pair2_eq_dec _ ty.Ty_eq_dec) in H2. *)
+    (*          subst; easy. *)
+    (*        - subst; easy. *)
+    (* Qed. *)
 
     Lemma peval_unop_sound {σ1 σ2} (op : UnOp σ1 σ2) (t : Term Σ σ1) :
       peval_unop op t ≡ term_unop op t.
     Proof.
       destruct op; cbn [peval_unop];
         auto using peval_unop'_sound, peval_not_sound.
+      all: auto.
     Qed.
 
     (* Definition peval_union {U K} (t : Term Σ (unionk_ty U K)) : Term Σ (ty.union U) := *)
